Add join_comm, join_assoc to simpset. Hopefully helpful stuff in CoCallCardinality

Launchbury/CoCallCardinality.thy
@@ -1,6 +1,76 @@
 theory CoCallCardinality
-imports FTreeCardinality CoCallAnalysis
+imports FTreeCardinality CoCallAnalysisBinds
 begin
+
+lemma subset_ccNeighbors:
+  "S \<subseteq> ccNeighbors {x} G \<longleftrightarrow> ccProd {x} S \<sqsubseteq> G"
+  by transfer (auto simp add: sym_def)
+
+lemma elem_ccNeighbors:
+  "xa \<in> ccNeighbors {x} G \<longleftrightarrow> (xa--x\<in>G)"
+  by transfer (auto simp add: sym_def)
+
+
+
+(*
+definition ccApprox :: "var ftree \<Rightarrow> CoCalls"
+  where "ccApprox t =  lub (ccFromList ` (paths t))"
+*)
+lift_definition ccApprox :: "var ftree \<Rightarrow> CoCalls"
+  is "\<lambda> xss .  lub (ccFromList ` xss)".
+
+lemma ccApprox_paths: "ccApprox t = lub (ccFromList ` (paths t))" by transfer simp
+
+lemma in_ccAppox: "(x--y\<in>(ccApprox t)) \<longleftrightarrow> (\<exists> xs \<in> paths t. (x--y\<in>(ccFromList xs)))"
+  unfolding ccApprox_paths
+  by transfer auto
+
+lemma ccApprox_mono: "paths t \<subseteq> paths t' \<Longrightarrow> ccApprox t \<sqsubseteq> ccApprox t'"
+  by (rule below_CoCallsI) (auto simp add: in_ccAppox)
+
+
+lemma ccFromList_below_ccApprox:
+  "xs \<in> paths t \<Longrightarrow> ccFromList xs \<sqsubseteq> ccApprox t" 
+by (rule below_CoCallsI)(auto simp add: in_ccAppox)
+
+lemma ccApprox_nxt_below:
+  "ccApprox (nxt t x) \<sqsubseteq> ccApprox t"
+by (rule below_CoCallsI)(auto simp add: in_ccAppox paths_nxt_eq elim!:  bexI[rotated])
+
+lemma interleave_ccFromList:
+  "xs \<in> interleave ys zs \<Longrightarrow> ccFromList xs = ccFromList ys \<squnion> ccFromList zs \<squnion> ccProd (set ys) (set zs)"
+  by (induction rule: interleave_induct)
+     (auto simp add: interleave_set ccProd_comm ccProd_insert2[where S' = "set xs" for xs]  ccProd_insert1[where S' = "set xs" for xs] )
+
+lemma ccApprox_both: "ccApprox (t \<otimes>\<otimes> t') = ccApprox t \<squnion> ccApprox t' \<squnion> ccProd (carrier t) (carrier t')"
+proof (rule below_antisym)
+  show "ccApprox (t \<otimes>\<otimes> t') \<sqsubseteq> ccApprox t \<squnion> ccApprox t' \<squnion> ccProd (carrier t) (carrier t')"
+    by (rule below_CoCallsI)
+       (auto 4 4  simp add: in_ccAppox paths_both Union_paths_carrier[symmetric]  interleave_ccFromList)
+next
+  have "ccApprox t \<sqsubseteq> ccApprox (t \<otimes>\<otimes> t')"
+    by (rule ccApprox_mono[OF both_contains_arg1])
+  moreover
+  have "ccApprox t' \<sqsubseteq> ccApprox (t \<otimes>\<otimes> t')"
+    by (rule ccApprox_mono[OF both_contains_arg2])
+  moreover
+  have "ccProd (carrier t) (carrier t') \<sqsubseteq> ccApprox (t \<otimes>\<otimes> t')"
+  proof(rule ccProd_belowI)
+    fix x y
+    assume "x \<in> carrier t" and "y \<in> carrier t'"
+    then obtain xs ys where "x \<in> set xs" and "y \<in> set ys"
+      and "xs \<in> paths t" and "ys \<in> paths t'" by (auto simp add: Union_paths_carrier[symmetric])
+    hence "xs @ ys \<in> paths (t \<otimes>\<otimes> t')" by (metis paths_both append_interleave)
+    moreover
+    from `x \<in> set xs` `y \<in> set ys`
+    have "x--y\<in>(ccFromList (xs@ys))" by simp
+    ultimately
+    show "x--y\<in>(ccApprox (t \<otimes>\<otimes> t'))" by (auto simp add: in_ccAppox simp del: ccFromList_append)
+  qed
+  ultimately
+  show "ccApprox t \<squnion> ccApprox t' \<squnion> ccProd (carrier t) (carrier t') \<sqsubseteq> ccApprox (t \<otimes>\<otimes> t')"
+    by (simp add: join_below_iff)
+qed
 
 definition aeFtree :: "AEnv \<Rightarrow> var ftree"
   where "aeFtree ae = many_among (edom ae)"
@@ -20,7 +90,6 @@ inductive_cases vald_lists_ConsE: "(x#xs) \<in> valid_lists S G"
 lemma  valid_lists_downset_aux:
   "xs \<in> valid_lists S CoCalls \<Longrightarrow> butlast xs \<in> valid_lists S CoCalls"
   by (induction xs) (auto dest: in_set_butlastD)
-
 
 lift_definition ccFTree :: "var set \<Rightarrow> CoCalls \<Rightarrow> var ftree" is "\<lambda> S G. valid_lists S G" 
   by (auto intro: valid_lists_downset_aux)
@@ -44,6 +113,87 @@ lemma carrier_ccFTree: "carrier (ccFTree S G) = S"
   apply (rule_tac x = "[x]" in bexI)
   apply auto
   done
+
+lemma ccProd_below_cc_restr:
+  "ccProd S S' \<sqsubseteq> cc_restr S'' G \<longleftrightarrow> ccProd S S' \<sqsubseteq> G \<and> (S = {} \<or> S' = {} \<or> S \<subseteq> S'' \<and> S' \<subseteq> S'')"
+  by transfer auto
+
+lemma valid_lists_ccFromList:
+  "xs \<in> valid_lists S G \<Longrightarrow> ccFromList xs \<sqsubseteq> cc_restr S G"
+by (induction rule:valid_lists.induct)
+   (auto simp add: join_below_iff subset_ccNeighbors ccProd_below_cc_restr elim: set_mp[OF valid_lists_subset])
+
+lemma ccApprox_ccFTree[simp]: "ccApprox (ccFTree S G) = cc_restr S G"
+proof (transfer' fixing: S G, rule below_antisym)
+  show "lub (ccFromList ` valid_lists S G) \<sqsubseteq> cc_restr S G"
+    apply (rule is_lub_thelub_ex)
+    apply (metis coCallsLub_is_lub)
+    apply (rule is_ubI)
+    apply clarify
+    apply (erule valid_lists_ccFromList)
+    done
+next
+  show "cc_restr S G \<sqsubseteq> lub (ccFromList ` valid_lists S G)"
+  proof (rule below_CoCallsI)
+    fix x y
+    have "x--y\<in>(ccFromList [y,x])" by simp
+    moreover
+    assume "x--y\<in>(cc_restr S G)"
+    hence "[y,x] \<in> valid_lists S G"  by (auto simp add: elem_ccNeighbors)
+    ultimately
+    show "x--y\<in>(lub (ccFromList ` valid_lists S G))"
+      by (rule in_CoCallsLubI[OF _ imageI])
+  qed
+qed
+
+lemma below_ccFTreeI:
+  assumes "carrier t \<subseteq> S" and "ccApprox t \<sqsubseteq> G"
+  shows "t \<sqsubseteq> ccFTree S G"
+unfolding paths_mono_iff[symmetric] below_set_def
+proof
+  fix xs
+  assume "xs \<in> paths t"
+  with assms
+  have "xs \<in> valid_lists S G"
+  proof(induction xs arbitrary : t)
+  case Nil thus ?case by simp
+  next
+  case (Cons x xs)
+    from `x # xs \<in> paths t`
+    have "possible t x" and "xs \<in> paths (nxt t x)" by (auto simp add: Cons_path)
+
+    have "ccProd {x} (set xs) \<sqsubseteq> ccFromList (x # xs)" by simp
+    also
+    from `x # xs \<in> paths t` 
+    have "\<dots> \<sqsubseteq> ccApprox t"
+      by (rule ccFromList_below_ccApprox)
+    also
+    note `ccApprox t \<sqsubseteq> G`
+    finally
+    have "ccProd {x} (set xs) \<sqsubseteq> G" by this simp_all
+    hence "set xs \<subseteq> ccNeighbors {x} G" unfolding subset_ccNeighbors.
+    moreover
+    have "xs \<in> valid_lists S G"
+    proof(rule Cons.IH)
+      show "xs \<in> paths (nxt t x)" by fact
+    next
+      from `carrier t \<subseteq> S`
+      show "carrier (nxt t x) \<subseteq> S" 
+        by (rule order_trans[OF carrier_nxt_subset])
+    next
+      from `ccApprox t \<sqsubseteq> G`
+      show "ccApprox (nxt t x) \<sqsubseteq> G" 
+        by (rule below_trans[OF ccApprox_nxt_below])
+    qed
+    moreover
+    from  `carrier t \<subseteq> S` and `possible t x`
+    have "x \<in> S" by (rule carrier_possible_subset)
+    ultimately
+    show ?case..
+  qed
+    
+  thus "xs \<in> paths (ccFTree S G)" by (metis paths_ccFTree)
+qed    
 
 lemma valid_lists_mono1:
   assumes "S \<subseteq> S'"
@@ -246,16 +396,112 @@ proof-
     show False..
   qed
 qed
+
+
+text {* An alternative definition *}
+
+inductive valid_lists' :: "var set \<Rightarrow> CoCalls \<Rightarrow> var set \<Rightarrow> var list \<Rightarrow> bool"
+  for S G
+  where  "valid_lists' S G prefix []"
+  | "prefix \<subseteq> ccNeighbors {x} G \<Longrightarrow> valid_lists' S G (insert x prefix) xs \<Longrightarrow> x \<in> S \<Longrightarrow> valid_lists' S G prefix (x#xs)"
+
+inductive_simps valid_lists'_simps[simp]: "valid_lists' S G prefix []" "valid_lists' S G prefix (x#xs)"
+inductive_cases vald_lists'_ConsE: "valid_lists' S G prefix (x#xs)"
+
+lemma valid_lists_valid_lists':
+  "xs \<in> valid_lists S G \<Longrightarrow> ccProd prefix (set xs) \<sqsubseteq> G \<Longrightarrow> valid_lists' S G prefix xs"
+proof(induction arbitrary: prefix rule: valid_lists.induct[case_names Nil Cons])
+  case Nil thus ?case by simp
+next
+  case (Cons xs x)
+
+  from Cons.prems Cons.hyps Cons.IH[where prefix = "insert x prefix"]
+  show ?case
+  by (auto simp add: insert_is_Un[where A = "set xs"]  insert_is_Un[where A = prefix]
+                     join_below_iff subset_ccNeighbors elem_ccNeighbors ccProd_comm simp del: Un_insert_left )
+qed
+
+lemma valid_lists'_valid_lists_aux:
+  "valid_lists' S G prefix xs \<Longrightarrow>  x \<in> prefix \<Longrightarrow> ccProd (set xs) {x} \<sqsubseteq> G"
+proof(induction  rule: valid_lists'.induct[case_names Nil Cons])
+  case Nil thus ?case by simp
+next
+  case (Cons prefix x xs)
+  thus ?case
+    apply (auto simp add: ccProd_insert2[where S' = prefix] ccProd_insert1[where S' = "set xs"] join_below_iff subset_ccNeighbors)
+    by (metis Cons.hyps(1) dual_order.trans empty_subsetI insert_subset subset_ccNeighbors)
+qed
+
+lemma valid_lists'_valid_lists:
+  "valid_lists' S G prefix xs \<Longrightarrow> xs \<in> valid_lists S G"
+proof(induction  rule: valid_lists'.induct[case_names Nil Cons])
+  case Nil thus ?case by simp
+next
+  case (Cons prefix x xs)
+  thus ?case
+    by (auto simp add: insert_is_Un[where A = "set xs"]  insert_is_Un[where A = prefix]
+                   join_below_iff subset_ccNeighbors elem_ccNeighbors ccProd_comm simp del: Un_insert_left 
+         intro: valid_lists'_valid_lists_aux)
+qed
+
+text {* Yet another definition *}
+
+lemma valid_lists_characterization:
+  "xs \<in> valid_lists S G \<longleftrightarrow> set xs \<subseteq> S \<and> (\<forall>n. ccProd (set (take n xs)) (set (drop n xs)) \<sqsubseteq> G)"
+proof(safe)
+  fix x
+  assume "xs \<in> valid_lists S G"
+  from  valid_lists_subset[OF this]
+  show "x \<in> set xs \<Longrightarrow> x \<in> S" by auto
+next
+  fix n
+  assume "xs \<in> valid_lists S G"
+  thus "ccProd (set (take n xs)) (set (drop n xs)) \<sqsubseteq> G"
+  proof(induction arbitrary: n rule: valid_lists.induct[case_names Nil Cons])
+    case Nil thus ?case by simp
+  next
+    case (Cons xs x)
+    show ?case
+    proof(cases n)
+      case 0 thus ?thesis by simp
+    next
+      case (Suc n)
+      with Cons.hyps Cons.IH[where n = n]
+      show ?thesis
+      apply (auto simp add: ccProd_insert1[where S' = "set xs" for xs] join_below_iff subset_ccNeighbors)
+      by (metis dual_order.trans set_drop_subset subset_ccNeighbors)
+    qed
+  qed
+next
+  assume "set xs \<subseteq> S"
+  and "\<forall> n. ccProd (set (take n xs)) (set (drop n xs)) \<sqsubseteq> G" 
+  thus "xs \<in> valid_lists S G"
+  proof (induction xs)
+    case Nil thus ?case by simp
+  next
+    case (Cons x xs)
+    from `\<forall>n. ccProd (set (take n (x # xs))) (set (drop n (x # xs))) \<sqsubseteq> G`
+    have "\<forall>n. ccProd (set (take n xs)) (set (drop n xs)) \<sqsubseteq> G"
+      by -(rule, erule_tac x = "Suc n" in allE, auto simp add: ccProd_insert1[where S' = "set xs" for xs] join_below_iff)
+    from Cons.prems Cons.IH[OF _ this]
+    have "xs \<in> valid_lists S G" by auto
+    with Cons.prems(1)  spec[OF `\<forall>n. ccProd (set (take n (x # xs))) (set (drop n (x # xs))) \<sqsubseteq> G`, where x = 1]
+    show ?case by (simp add: subset_ccNeighbors)
+  qed
+qed
   
+
 
 locale CoCallCardinality = CoCallAnalysis + CoCallAnalyisHeap + CorrectArityAnalysisLet' +
   assumes ccExp_App: "ccExp e\<cdot>(inc\<cdot>a) \<squnion> ccProd {x} (insert x (fv e)) \<sqsubseteq> ccExp (App e x)\<cdot>a"
   assumes ccExp_Lam: "cc_restr (fv (Lam [y]. e)) (ccExp e\<cdot>(pred\<cdot>n)) \<sqsubseteq> ccExp (Lam [y]. e)\<cdot>n"
   assumes ccExp_subst: "x \<notin>  S \<Longrightarrow> y \<notin> S \<Longrightarrow> cc_restr S (ccExp e[y::=x]\<cdot>a) \<sqsubseteq> cc_restr S (ccExp e\<cdot>a)"
   assumes ccExp_pap: "isLam e \<Longrightarrow> ccExp e\<cdot>0 = ccSquare (fv e)"
+  assumes ccExp_Let: "ccBindsExtra \<Gamma>\<cdot>(Aheap \<Gamma> e\<cdot>a, ccHeap \<Gamma> e\<cdot>a) \<squnion> ccExp e\<cdot>a \<sqsubseteq> ccHeap \<Gamma> e\<cdot>a \<squnion> ccExp (Let \<Gamma> e)\<cdot>a"
  
   assumes aHeap_thunks: "x \<in> thunks \<Gamma> \<Longrightarrow> x \<in> edom (Aheap \<Gamma> e\<cdot>a) \<Longrightarrow> x \<in> ccManyCalls (ccHeap \<Gamma> e\<cdot>a) \<Longrightarrow> (Aheap \<Gamma> e\<cdot>a) x = up\<cdot>0"
 begin
+
 
 definition Fexp :: "exp \<Rightarrow> Arity \<rightarrow> var ftree"
   where "Fexp e = (\<Lambda> a. ccFTree (edom (Aexp e \<cdot>a)) (ccExp e\<cdot>a))"
@@ -290,14 +536,8 @@ proof default
     by (rule interleave_ccFTree)
   also have "\<dots> \<sqsubseteq> ccFTree (edom (Aexp (App e x)\<cdot>a)) (ccProd {x} {x} \<squnion> ccExp e\<cdot>(inc\<cdot>a) \<squnion> ccProd {x} (edom (Aexp e\<cdot>(inc\<cdot>a))))"
     by (rule ccFTree_mono1[OF *])
-  also have "ccProd {x} {x} \<squnion> ccExp e\<cdot>(inc\<cdot>a) \<squnion> ccProd {x} (edom (Aexp e\<cdot>(inc\<cdot>a))) = ccExp e\<cdot>(inc\<cdot>a) \<squnion> (ccProd {x} {x} \<squnion> ccProd {x} (edom (Aexp e\<cdot>(inc\<cdot>a))))"
-    apply (rule trans[OF join_assoc])
-    apply (rule trans[OF join_comm])
-    apply (rule trans[OF join_assoc])
-    apply (rule arg_cong[OF join_comm])
-    done
-  also have "\<dots> = ccExp e\<cdot>(inc\<cdot>a) \<squnion> ccProd {x} ({x} \<union> (edom (Aexp e\<cdot>(inc\<cdot>a))))"
-    by (simp add:  ccProd_union[symmetric] del: ccProd_union)
+  also have "ccProd {x} {x} \<squnion> ccExp e\<cdot>(inc\<cdot>a) \<squnion> ccProd {x} (edom (Aexp e\<cdot>(inc\<cdot>a))) = ccExp e\<cdot>(inc\<cdot>a) \<squnion> ccProd {x} ({x} \<union> (edom (Aexp e\<cdot>(inc\<cdot>a))))"
+    by (simp add: ccProd_union2[symmetric] del: ccProd_union2)
   also have "ccProd {x} ({x} \<union> (edom (Aexp e\<cdot>(inc\<cdot>a)))) \<sqsubseteq> ccProd {x} (insert x (fv e))"
     by (rule ccProd_mono2[OF **])
   also have "ccExp e\<cdot>(inc\<cdot>a) \<squnion> ccProd {x} (insert x (fv e)) \<sqsubseteq> ccExp (App e x)\<cdot>a"
@@ -377,11 +617,131 @@ definition Fheap :: "heap \<Rightarrow> exp \<Rightarrow> Arity \<rightarrow> va
 lemma Fheap_simp: "Fheap \<Gamma> e\<cdot>a = ccFTree (edom (Aheap \<Gamma> e\<cdot>a)) (ccHeap \<Gamma> e\<cdot>a)"
   unfolding Fheap_def sorry
 
+lemma carrier_Fheap:"carrier (Fheap \<Gamma> e\<cdot>a) = edom (Aheap \<Gamma> e\<cdot>a)"
+    unfolding Fheap_simp carrier_ccFTree.. 
+
+lemma carrier_substitute_aux:
+  assumes "xs \<in> paths (substitute f T t)"
+  assumes "carrier t \<subseteq> A"
+  assumes "\<And> x. x \<in> A \<Longrightarrow> carrier (f x) \<subseteq> A" 
+  shows   "set xs \<subseteq> A"
+  using assms
+  apply(induction  f T t xs rule: substitute_induct)
+  apply auto
+  apply (metis carrier_possible_subset)
+  apply (metis carrier_f_nxt carrier_nxt_subset carrier_possible_subset contra_subsetD order_trans)
+  done
+
+term substitute''
+lemma ccApprox_substitute_aux:
+  
+  assumes "substitute'' f T xs ys"
+  assumes "ccFromList (prefix@xs) \<sqsubseteq> G"
+  assumes "\<And> x. x \<in> set ys \<Longrightarrow> ccApprox (f x) \<sqsubseteq> G" 
+  shows   "ccFromList (prefix@ys) \<sqsubseteq> G"
+using assms
+proof(induction f T xs ys arbitrary: prefix rule: substitute''.induct[case_names Nil Cons])
+  case Nil thus ?case by simp
+next
+  case (Cons zs f x xs' xs T ys)
+  from `ccFromList (prefix @ x # xs) \<sqsubseteq> G`
+  have  "ccFromList prefix \<sqsubseteq> G"
+    and "ccProd (set prefix) (insert x (set xs)) \<sqsubseteq> G"
+    and "ccProd {x} (set xs) \<sqsubseteq> G"
+    and "ccFromList xs \<sqsubseteq> G"
+    by (auto simp add: join_below_iff)
+
+  from Cons have "ccApprox (f x) \<sqsubseteq> G" and *: "\<And>x. x \<in> set ys \<Longrightarrow> ccApprox (f x) \<sqsubseteq> G" by auto
+  with Cons.hyps(1)
+  have "ccFromList zs \<sqsubseteq> G" by (metis below_trans ccFromList_below_ccApprox) 
+  
+  have "ccFromList ((prefix@[x])@ys) \<sqsubseteq> G"
+  proof (rule Cons.IH)
+    have "ccProd {x} (set zs) \<sqsubseteq> G" sorry
+    moreover
+    have "ccFromList zs \<sqsubseteq> G" by fact
+    moreover
+    have "ccProd (set xs) (set zs) \<sqsubseteq> G" sorry
+    moreover
+    have "ccProd (set prefix) (set zs) \<sqsubseteq> G" sorry
+    moreover
+    note `ccFromList (prefix @ x # xs) \<sqsubseteq> G`
+    ultimately
+    show "ccFromList ((prefix @ [x]) @ xs') \<sqsubseteq> G"    
+      using interleave_ccFromList[OF `xs' \<in> xs \<otimes> zs`] interleave_set[OF  `xs' \<in> xs \<otimes> zs`]
+          by (auto simp add: ccApprox_both join_below_iff ccProd_insert2[where S' = "S \<union> S'" for S S'] ccProd_insert2[where S' = "set xs" for xs])
+  next
+    fix x'
+    assume "x' \<in> set ys"
+    thus "ccApprox (f_nxt f T x x') \<sqsubseteq> G" sorry
+  qed
+  moreover
+  thm Cons
+  have "ccProd {x} (set ys) \<sqsubseteq> G" sorry
+  ultimately
+  show ?case by simp
+qed
+
+lemma ccFTree_Let:
+ "ccFTree (edom (ABinds \<Delta>\<cdot>(Aheap \<Delta> e\<cdot>a) \<squnion> Aexp e\<cdot>a)) (ccBindsExtra \<Delta>\<cdot>(Aheap \<Delta> e\<cdot>a, ccHeap \<Delta> e\<cdot>a) \<squnion> ccExp e\<cdot>a) \<sqsubseteq>
+  ccFTree (edom (Aheap \<Delta> e\<cdot>a \<squnion> Aexp (Let \<Delta> e)\<cdot>a)) (ccHeap \<Delta> e\<cdot>a \<squnion> ccExp (Let \<Delta> e)\<cdot>a)"
+ using Aexp_Let[of \<Delta> e a] ccExp_Let[of \<Delta> e a]
+ by (rule below_trans[OF ccFTree_mono1[OF edom_mono] ccFTree_mono2])
+
+lemma substitute'_valid_list:
+  assumes "xs \<in> paths (substitute f (thunks \<Delta>) t)"
+  assumes "f = env_restr (- (S \<inter> thunks \<Delta>)) (Fexp.AnalBinds \<Delta>\<cdot>(Aheap \<Delta> e\<cdot>a))" 
+  assumes "ccProd (carrier t) S \<sqsubseteq> ccBindsExtra \<Delta>\<cdot>(Aheap \<Delta> e\<cdot>a, ccHeap \<Delta> e\<cdot>a) \<squnion> ccExp e\<cdot>a"
+  shows   "valid_lists' (edom (ABinds \<Delta>\<cdot>(Aheap \<Delta> e\<cdot>a) \<squnion> Aexp e\<cdot>a)) (ccBindsExtra \<Delta>\<cdot>(Aheap \<Delta> e\<cdot>a, ccHeap \<Delta> e\<cdot>a) \<squnion> ccExp e\<cdot>a) S xs"
+using assms
+proof(induction  f "thunks \<Delta>" t xs arbitrary: S rule: substitute_induct)
+  case Nil
+  thus ?case by simp
+next
+  case (Cons f t x xs)
+
+  from `x # xs \<in> paths (substitute f (thunks \<Delta>) t)`
+  have "possible t x" and "xs \<in> paths (substitute (f_nxt f (thunks \<Delta>) x) (thunks \<Delta>) (nxt t x \<otimes>\<otimes> f x))"
+    by auto
+
+  note this(2)
+  moreover
+
+  have [simp]: "(- {x} \<inter> (- S \<union> - thunks \<Delta>)) = (- insert x (S \<inter> thunks \<Delta>))" by auto
+    
+  from  Cons.prems(2)
+  have "f_nxt f (thunks \<Delta>) x = env_restr (-(insert x S \<inter> thunks \<Delta>)) (ExpAnalysis.AnalBinds Fexp \<Delta>\<cdot>(Aheap \<Delta> e\<cdot>a))"
+    by (cases "x \<in> thunks \<Delta>")
+       (auto simp add: f_nxt_def env_delete_def[symmetric] empty_is_bottom env_delete_restr)
+  moreover
+  from below_trans[OF ccProd_mono1[OF carrier_nxt_subset] `ccProd (carrier t) _ \<sqsubseteq> _`]
+  have "ccProd (carrier (nxt t x \<otimes>\<otimes> f x)) (insert x S) \<sqsubseteq> ccBindsExtra \<Delta>\<cdot>(Aheap \<Delta> e\<cdot>a, ccHeap \<Delta> e\<cdot>a) \<squnion> ccExp e\<cdot>a" 
+    apply (auto simp add: join_below_iff ccProd_insert2[where S' = S])
+    thm ccProd_mono1[OF carrier_nxt_subset]
+    sorry
+  ultimately
+  have IH: "valid_lists' (edom (ABinds \<Delta>\<cdot>(Aheap \<Delta> e\<cdot>a) \<squnion> Aexp e\<cdot>a)) (ccBindsExtra \<Delta>\<cdot>(Aheap \<Delta> e\<cdot>a, ccHeap \<Delta> e\<cdot>a) \<squnion> ccExp e\<cdot>a) (insert x S) xs"  
+    by (rule Cons.hyps)
+
+  have "x \<in> carrier t" by (metis `possible t x` carrier_possible)
+  hence "ccProd {x} S \<sqsubseteq> ccProd (carrier t) S" by (auto intro: ccProd_mono1)
+  with `ccProd (carrier t) _ \<sqsubseteq> _`
+  have "S \<subseteq> ccNeighbors {x} (ccBindsExtra \<Delta>\<cdot>(Aheap \<Delta> e\<cdot>a, ccHeap \<Delta> e\<cdot>a) \<squnion> ccExp e\<cdot>a)"
+    unfolding subset_ccNeighbors
+    by (rule below_trans[rotated])
+  moreover
+  note IH
+  moreover
+  have "x \<in> edom (ABinds \<Delta>\<cdot>(Aheap \<Delta> e\<cdot>a) \<squnion> Aexp e\<cdot>a)" sorry
+  ultimately
+  show ?case..
+qed
+
 sublocale FutureAnalysisCardinalityHeap Fexp Aexp Aheap Fheap
 proof default
   fix \<Gamma> e a
   show "carrier (Fheap \<Gamma> e\<cdot>a) = edom (Aheap \<Gamma> e\<cdot>a)"
-    unfolding Fheap_simp carrier_ccFTree..
+    by (rule carrier_Fheap)
 next
   fix x \<Gamma> p e a
   assume "x \<in> thunks \<Gamma>"
@@ -395,9 +755,48 @@ next
     by (rule aHeap_thunks)
 next
   fix \<Delta> e a
-  show "ftree_restr (domA \<Delta>) (substitute (Fexp.AnalBinds \<Delta>\<cdot>(Aheap \<Delta> e\<cdot>a)) (Fexp e\<cdot>a)) \<sqsubseteq> Fheap \<Delta> e\<cdot>a"
-    unfolding Fheap_simp Fexp_simp
-  find_theorems ftree_restr substitute
+
+  have "substitute (Fexp.AnalBinds \<Delta>\<cdot>(Aheap \<Delta> e\<cdot>a)) (thunks \<Delta>) (Fexp e\<cdot>a) \<sqsubseteq> 
+        ccFTree (edom (ABinds \<Delta>\<cdot>(Aheap \<Delta> e\<cdot>a) \<squnion> Aexp e\<cdot>a)) (ccBindsExtra \<Delta>\<cdot>(Aheap \<Delta> e\<cdot>a, ccHeap \<Delta> e\<cdot>a) \<squnion> ccExp e\<cdot>a)"
+  unfolding paths_mono_iff[symmetric] below_set_def
+  proof
+    fix xs
+    assume "xs \<in> paths (substitute (Fexp.AnalBinds \<Delta>\<cdot>(Aheap \<Delta> e\<cdot>a)) (thunks \<Delta>) (Fexp e\<cdot>a))"
+    hence "set xs \<subseteq> edom (ABinds \<Delta>\<cdot>(Aheap \<Delta> e\<cdot>a) \<squnion> Aexp e\<cdot>a)"
+    proof (rule carrier_substitute_aux)
+      show "carrier (Fexp e\<cdot>a) \<subseteq> edom (ABinds \<Delta>\<cdot>(Aheap \<Delta> e\<cdot>a) \<squnion> Aexp e\<cdot>a)"
+       by (auto simp add: Fexp_simp carrier_ccFTree)
+    next
+      fix x
+      have "carrier ((Fexp.AnalBinds  \<Delta>\<cdot>(Aheap \<Delta> e\<cdot>a)) x) \<subseteq> edom (ABinds \<Delta>\<cdot>(Aheap \<Delta> e\<cdot>a))"
+      apply (auto simp add: Fexp.AnalBinds_lookup Fexp_simp split: option.split)
+      apply (cases "(Aheap \<Delta> e\<cdot>a) x") 
+      apply (auto simp add: Fexp_simp carrier_ccFTree elim: set_mp[OF edom_mono[OF monofun_cfun_fun[OF ABind_below_ABinds]]])
+      done
+      thus "carrier ((Fexp.AnalBinds  \<Delta>\<cdot>(Aheap \<Delta> e\<cdot>a)) x) \<subseteq> edom (ABinds \<Delta>\<cdot>(Aheap \<Delta> e\<cdot>a) \<squnion> Aexp e\<cdot>a)" by auto
+    qed
+
+    have "xs \<in> valid_lists (edom (ABinds \<Delta>\<cdot>(Aheap \<Delta> e\<cdot>a) \<squnion> Aexp e\<cdot>a)) (ccBindsExtra \<Delta>\<cdot>(Aheap \<Delta> e\<cdot>a, ccHeap \<Delta> e\<cdot>a) \<squnion> ccExp e\<cdot>a)" sorry
+    thus "xs \<in> paths (ccFTree (edom (ABinds \<Delta>\<cdot>(Aheap \<Delta> e\<cdot>a) \<squnion> Aexp e\<cdot>a)) (ccBindsExtra \<Delta>\<cdot>(Aheap \<Delta> e\<cdot>a, ccHeap \<Delta> e\<cdot>a) \<squnion> ccExp e\<cdot>a))"
+      by (transfer fixing: ccExp Aexp Aheap ccHeap)
+  qed
+  also
+  note ccFTree_Let
+  finally
+  have "substitute (ExpAnalysis.AnalBinds Fexp \<Delta>\<cdot>(Aheap \<Delta> e\<cdot>a)) (thunks \<Delta>) (Fexp e\<cdot>a) \<sqsubseteq>
+        ccFTree (edom (Aheap \<Delta> e\<cdot>a \<squnion> Aexp (Terms.Let \<Delta> e)\<cdot>a)) (ccHeap \<Delta> e\<cdot>a \<squnion> ccExp (Terms.Let \<Delta> e)\<cdot>a)" (is "_ \<sqsubseteq> ?R") by this simp
+  
+  moreover
+  have  "ftree_restr (domA \<Delta>) ?R = Fheap \<Delta> e\<cdot>a"
+   and "ftree_restr (- domA \<Delta>) ?R = Fexp (Let \<Delta> e)\<cdot>a"
+   apply (auto simp add: Fheap_simp Fexp_simp)
+    sorry
+    by (auto intro!: ftree_restr_is_empty ftree_restr_noop  dest!: set_mp[OF carrier_Fexp] simp add: carrier_Fheap dest: set_mp[OF edom_Aheap])
+  ultimately
+  show "ftree_restr (domA \<Delta>) (substitute (Fexp.AnalBinds \<Delta>\<cdot>(Aheap \<Delta> e\<cdot>a)) (thunks \<Delta>)  (Fexp e\<cdot>a)) \<sqsubseteq> Fheap \<Delta> e\<cdot>a"
+  and  "ftree_restr (- domA \<Delta>) (substitute (Fexp.AnalBinds \<Delta>\<cdot>(Aheap \<Delta> e\<cdot>a)) (thunks \<Delta>)  (Fexp e\<cdot>a)) \<sqsubseteq> Fexp (Let \<Delta> e)\<cdot>a"
+    by (metis  ftree_restr_mono)+
+qed
 
 end
 
